Heap/MoveDown.v
@@ -1,0 +1,41 @@
+Require Import Coq.Lists.List.
+Require Import Coq.ZArith.ZArith.
+Require Import Coq.Classes.RelationClasses.
+Require Import PL.Monad.
+Require Import PL.Monad2.
+Require Import SetsClass.
+Require Import HEAP.Defs.
+Import SetsNotation
+       StateRelMonad
+       StateRelMonadOp
+       StateRelMonadHoare
+       MonadNotation
+       Monad.
+Local Open Scope sets.
+Local Open Scope Z.
+Local Open Scope monad.
+
+(* 下移节点操作正确性：
+1. 集合不变
+2. 保持二叉树合法性
+3. 从堆或局部破坏的堆开始，最终恢复堆性质
+4. 保持满二叉树 *)
+
+Theorem move_down_correctness1: forall (v: Z) (V: Z -> Prop),
+  Hoare (fun s => s.(heap).(vvalid) v /\
+                  Abs s.(heap) V /\
+                  BinaryTree.legal s.(heap) /\
+                  (Heap_broken_down s.(heap) v \/ Heap s.(heap)))
+        (move_down v)
+        (fun _ s => Abs s.(heap) V /\
+                    BinaryTree.legal s.(heap) /\
+                    Heap s.(heap)).
+Admitted.
+
+Theorem move_down_correctness2: forall (v: Z),
+  Hoare (fun s => s.(heap).(vvalid) v /\
+                  BinaryTree.legal s.(heap) /\
+                  is_complete_or_full_bintree s.(heap))
+        (move_down v)
+        (fun _ s => is_complete_or_full_bintree s.(heap)).
+Admitted.
